theories/Prelude/PreludeMath.v
@@ -180,6 +180,30 @@ Module MathProps.
     }
   .
 
+  Section DOMAIN_THEORIC_CONCEPTS.
+
+  Local Notation " x '>=' y " := (leProp y x) (only parsing, at level 70, no associativity) : type_scope.
+
+  Definition PrefixedPoints {D : Type} {requiresPoset : isPoset D} (f : D -> D) : ensemble D := fun x : D => (x >= f x)%type.
+
+  Definition FixedPoints {D : Type} {requiresSetoid : isSetoid D} (f : D -> D) : ensemble D := fun x : D => (x == f x)%type.
+
+  Definition PostfixedPoints {D : Type} {requiresPoset : isPoset D} (f : D -> D) : ensemble D := fun x : D => (x =< f x)%type.
+
+  Definition UpperBoundsOf {D : Type} {requiresPoset : isPoset D} (X : ensemble D) : ensemble D := fun upper_bound : D => forall x : D, << H_IN : member x X >> -> (x =< upper_bound)%type.
+
+  Definition LowerBoundsOf {D : Type} {requiresPoset : isPoset D} (X : ensemble D) : ensemble D := fun lower_bound : D => forall x : D, << H_IN : member x X >> -> (x >= lower_bound)%type.
+
+  Definition isSupremumOf {D : Type} {requiresPoset : isPoset D} (sup_X : D) (X : ensemble D) : Prop :=
+    forall upper_bound : D, << SUPREMUM_LE_UPPER_BOUND : (sup_X =< upper_bound)%type >> <-> << UPPER_BOUND : member upper_bound (UpperBoundsOf X) >>
+  .
+
+  Definition isInfimumOf {D : Type} {requiresPoset : isPoset D} (inf_X : D) (X : ensemble D) : Prop :=
+    forall lower_bound : D, << LOWER_BOUND_LE_INFIMUM : (inf_X >= lower_bound)%type >> <-> << LOWER_BOUND : member lower_bound (LowerBoundsOf X) >>
+  .
+
+  End DOMAIN_THEORIC_CONCEPTS.
+
 End MathProps.
 
 Export MathProps.
@@ -698,14 +722,6 @@ Module MathClasses.
     }
   .
 
-  Definition UpperBoundOf {D : Type} {requiresPoset : isPoset D} (X : ensemble D) : ensemble D :=
-    fun upper_bound : D => forall x : D, << H_IN : member x X >> -> x =< upper_bound
-  .
-
-  Definition isSupremumOf {D : Type} {requiresPoset : isPoset D} (sup_X : D) (X : ensemble D) : Prop :=
-    forall upper_bound : D, << SUPREMUM_LE_UPPER_BOUND : sup_X =< upper_bound >> <-> << UPPER_BOUND : member upper_bound (UpperBoundOf X) >>
-  .
-
   Definition isDirectedSubset {D : Type} {requiresPoset : isPoset D} (X : ensemble D) : Prop :=
     forall x1 : D, << H_IN1 : member x1 X >> ->
     forall x2 : D, << H_IN2 : member x2 X >> ->
@@ -764,13 +780,5 @@ Module MathClasses.
   Proof. now eapply partial_order_equivalence. Qed.
 
   End BASIC_POSET_THEORY.
-
-  Local Notation " x '>=' y " := (leProp y x) (only parsing, at level 70, no associativity) : type_scope.
-
-  Definition PreFixedPoints {D : Type} {requiresPoset : isPoset D} (f : D -> D) : ensemble D := fun x : D => (x >= f x)%type.
-
-  Definition FixedPoints {D : Type} {requiresSetoid : isSetoid D} (f : D -> D) : ensemble D := fun x : D => (x == f x)%type.
-
-  Definition PostFixedPoints {D : Type} {requiresPoset : isPoset D} (f : D -> D) : ensemble D := fun x : D => (x =< f x)%type.
 
 End MathClasses.
